devel/Iron/Language/DelayedSystemF/TypeX.v
@@ -1,26 +1,38 @@
 
 Require Export Iron.Language.DelayedSystemF.Exp.
+Require Export Iron.Language.DelayedSystemF.SubstTT.
 
 
 (*******************************************************************)
 (* Typing judgement assigns a type to an expression. *)
-Inductive TypeX : tyenv -> exp -> ty -> Prop :=
+Inductive TypeX : kienv -> tyenv -> exp -> ty -> Prop :=
  | TxVar 
-   :  forall te v t
+   :  forall ke te v t
    ,  lookupEnv v te = Some t
-   -> TypeX te (XVar v) t
+   -> TypeX  ke te (XVar v) t
 
- | TxLam
-   :  forall te ss v1 t1 x2 t2
-   ,  ForallSubstXT (TypeX te) ss
-   -> TypeX (te >< stripS ss :> SSig v1 t1) x2 t2
-   -> TypeX te (XAbs ss v1 t1 x2) (TFun t1 t2)
+ | TxAbs
+   :  forall ke te sx v1 t1 x2 t2
+   ,  ForallSubstXT (TypeX ke te) sx
+   -> TypeX  ke (te >< stripS sx :> SSig v1 t1) x2 t2
+   -> TypeX  ke te (XAbs sx v1 t1 x2) (TFun t1 t2)
 
+ (* TODO need type equiv here, rather than just t1 *)
  | TxApp
-   :  forall te x1 x2 t1 t2
-   ,  TypeX te x1 (TFun t1 t2)
-   -> TypeX te x2 t1
-   -> TypeX te (XApp x1 x2) t2.
+   :  forall ke te x1 x2 t1 t2
+   ,  TypeX  ke te x1 (TFun t1 t2)
+   -> TypeX  ke te x2 t1
+   -> TypeX  ke te (XApp x1 x2) t2
+
+ | TxABS
+   :  forall ke te st sx a1 k1 x2 t2
+   ,  TypeX  (ke >< stripS st :> SSig a1 k1) (te >< stripS sx) x2 t2
+   -> TypeX  ke te (XABS st sx a1 k1 x2) (TForall st a1 k1 t2)
+
+ | TxAPP
+   :  forall ke te st a1 k1 t1 x1 t2
+   ,  TypeX  ke te x1 (TForall st a1 k1 t1)
+   -> TypeX  ke te (XAPP x1 t2) (substTT (st :> BBind a1 k1 t2) t1).
 
 Hint Constructors TypeX.
 
@@ -29,48 +41,15 @@ Hint Constructors TypeX.
 Ltac inverts_type :=
  repeat 
   (match goal with 
-   | [ H: TypeX _ (XVar _) _       |- _ ] => inverts H
-   | [ H: TypeX _ (XAbs _ _ _ _) _ |- _ ] => inverts H
-   | [ H: TypeX _ (XApp _ _) _     |- _ ] => inverts H
+   | [ H: TypeX _ _ (XVar _) _         |- _ ] => inverts H
+   | [ H: TypeX _ _ (XAbs _ _ _ _) _   |- _ ] => inverts H
+   | [ H: TypeX _ _ (XApp _ _) _       |- _ ] => inverts H
+   | [ H: TypeX _ _ (XABS _ _ _ _ _) _ |- _ ] => inverts H
+   | [ H: TypeX _ _ (XAPP _ _) _       |- _ ] => inverts H
    end).
 
 
 (* Closed expressions are well typed under an empty environment. *)
 Definition Closed (xx: exp) : Prop := 
- exists t, TypeX nil xx t.
-
-
-(*******************************************************************)
-(* Forms of terms lemma. *)
-Lemma done_lam 
- :  forall x t1 t2
- ,  TypeX nil x (TFun t1 t2)
- -> Done   x
- -> isXAbs x.
-Proof.
- intros. gen t1 t2.
- induction x; intros.
-
- - Case "XVar".
-   nope.
-
- - Case "XAbs".
-   nope.
-
- - Case "XApp".
-   inverts H0.
-   + nope.
-
-   + destruct x1.
-     * nope.
-
-     * rip.
-       assert (Value (XAbs ss v t x1)); auto.
-       nope.
-
-     * inverts_type.
-       rip.
-       assert (isXAbs (XApp x1_1 x1_2)).
-        eapply IHx1. eauto. nope.
-Qed.
+ exists t, TypeX nil nil xx t.
 
