devel/Iron/Language/DelayedSystemF/Progress.v
@@ -5,17 +5,17 @@ Require Export Iron.Language.DelayedSystemF.Step.
 (* A well typed expression is either a value or can 
    take a step in the evaluation. *)
 Theorem progress
- :  forall te x t
- ,  TypeX  te x t
+ :  forall ke te x t
+ ,  TypeX  ke te x t
  -> Done x \/ (exists x', Step x x').
 Proof.
  intros. gen t.
  induction x using exp_iind; intros.
 
- - Case "XVar".
+ - Case "XVar is done".
    left. auto.
 
- - Case "XLam".
+ - Case "XLam is done".
    left. auto.
 
  - Case "XApp".
@@ -25,37 +25,27 @@ Proof.
    destruct HX1.
 
    + SCase "x1 is done.".
-     destruct x1.
+     destruct x1; firstorder.
 
-     * SSCase "x1 is a variable".
-       left.  eapply DoneApp. 
-       split. 
-        eapply DoneVar.
-        intuition. nope.
-
-     * SSCase "x1 is a lambda".
+     * SSCase "x1 is an abstraction".
        right.
        assert (Done x2 \/ (exists x2', Step x2 x2')) as HX2; eauto.
        destruct HX2.
 
        SSSCase "beta reduction".
-        exists (substXX (BBind v t0 x2 :: ss) x1).
+        exists (substXX (BBind v t0 x2 :: sx) x1).
         eapply EsAbsApp.
         assumption.
 
        SSSCase "x2 steps".
         destruct H0 as [x2'].
-        exists (XApp (XAbs ss v t0 x1) x2').
+        exists (XApp (XAbs sx v t0 x1) x2').
         eapply EsAppRight.
          inverts H. assumption.
          assumption.
 
-     * SSCase "x1 is an application".
-       left.
-       eapply DoneApp.
-       split.
-        assumption.
-        intuition. nope.
+     * SSCase "x1 is a type abstraction".
+       nope.
 
    + SCase "x1 steps".
      destruct H as [x1'].
@@ -63,5 +53,32 @@ Proof.
      exists (XApp x1' x2).
      eapply EsAppLeft.
      assumption.
+
+ - Case "XABS is done".
+   left. auto.
+
+ - Case "XAPP".
+   inverts_type.
+
+   assert (Done x \/ (exists x', Step x x')) as HX; eauto.
+   destruct HX.
+
+   + SCase "x1 is done".
+     destruct x; firstorder.
+
+     * SSCase "x1 is an abstraction".
+       nope.
+
+     * SSCase "x1 is a type abstraction".
+       right.
+       exists (substTX (st0 :> BBind a k t2) sx x).
+       eapply EsABSAPP.
+
+  + SCase "x1 steps".
+    destruct H as [x'].
+    right.
+    exists (XAPP x' t2).
+    eapply EsAPPLeft.
+    assumption.
 Qed.
 
