devel/Iron/Language/DelayedSystemF/SubstTT.v
@@ -1,0 +1,22 @@
+
+Require Export Iron.Language.DelayedSystemF.Ty.
+
+
+(* Apply an type substitution to a type. *)
+Fixpoint substTT (ss: @subst ty ki) (tt: ty) {struct tt} : ty  :=
+ match tt with
+ |  TCon c
+ => tt
+
+ |  TVar a
+ => match lookupSubst a ss with
+    | None                => tt
+    | Some (BBind _ _ t)  => t
+    end
+
+ |  TForall ss2 a k t
+ => TForall (ss >< mapExpOfSubst (substTT ss) ss2) a k t
+
+ |  TFun t1 t2
+ => TFun (substTT ss t1) (substTT ss t2)
+ end.
