devel/Iron/Language/DelayedSystemF/SubstXX.v
@@ -11,33 +11,34 @@ Fixpoint substXX (ss: @subst exp ty) (xx: exp) {struct xx} : exp  :=
     | Some (BBind _ _ x)  => x
     end
 
- |  XAbs ss2 n t x
- => XAbs (ss >< mapExpOfSubst (substXX ss) ss2) n t x
+ |  XAbs sx n t x
+ => XAbs (ss >< mapExpOfSubst (substXX ss) sx) n t x
 
  |  XApp x1 x2
  => XApp (substXX ss x1) (substXX ss x2)
+
+ |  XABS st sx a k x
+ => XABS st (ss >< mapExpOfSubst (substXX ss) sx) a k x
+
+ |  XAPP x1 t2 
+ => XAPP (substXX ss x1) t2
  end.
 
 
-(* Substitution of expressions in expressions preserves typing.
-
-   Inductively, we must reason about performing substitutions at any
-   depth, hence we must prove a property about (subst' d x2 x1) instead
-   of the weaker (subst x2 x1) which assumes the substitution is taking
-   place at top level. 
-*)
+(* Substitution of expressions in expressions preserves typing. *)
 Lemma subst_exp_exp
- :  forall te ss x t
- ,  TypeX  (te >< stripS ss) x t
- -> ForallSubstXT (TypeX te) ss
- -> TypeX  te (substXX ss x) t.
+ :  forall ke te sx x t
+ ,  TypeX  ke (te >< stripS sx) x t
+ -> ForallSubstXT (TypeX ke te) sx
+ -> TypeX  ke te (substXX sx x) t.
 Proof.
- intros. gen te ss t.
+ intros. gen ke te sx t.
  induction x using exp_iind;
-  intros; simpl in *; inverts_type.
+  intros; simpl in *.
 
  - Case "XVar".
-   remember (lookupSubst n ss) as o.
+   inverts_type.
+   remember (lookupSubst n sx) as o.
    symmetry in Heqo.
    destruct o.
 
@@ -54,18 +55,20 @@ Proof.
      eapply TxVar.
      eapply lookup_env_subst_none; eauto.
 
- - Case "XLam".
-   eapply TxLam.
+ - Case "XAbs".
+   inverts_type.
+   eapply TxAbs.
    + eapply ForallSubstXT_app; auto.
 
+     eapply (Forall_inst ke)  in H.
      eapply (Forall_inst te)  in H.
-     eapply (Forall_inst ss0) in H.
+     eapply (Forall_inst sx0) in H.
      eapply (Forall_mp_const) in H; auto.
 
      eapply (Forall_map 
               (  fun xx => forall t
-              ,  TypeX (te >< stripS ss0) xx t
-              -> TypeX te (substXX ss0 xx) t)) in H.
+              ,  TypeX ke (te >< stripS sx0) xx t
+              -> TypeX ke te (substXX sx0 xx) t)) in H.
 
      eapply Forall_Forall2_right  in H.
      eapply ForallSubstXT_fold    in H.
@@ -81,6 +84,25 @@ Proof.
      assumption.
 
  - Case "XApp".
+   inverts_type.
    eapply TxApp; eauto.
+
+ - Case "XABS".
+   destruct t; nope.
+   destruct k. destruct k0.
+   inverts_type.
+   eapply TxABS.
+   unfold stripS.
+   rewrite map_app.
+   repeat (rewrite stripS_fold).
+   rewrite stripS_mapExpOfSubst.
+   rewrite <- app_assoc.
+   destruct k1.
+   assumption.
+
+ - Case "XAPP".
+   inverts_type.
+   eapply TxAPP.
+   eapply IHx; auto.
 Qed.
 
